---
title: "Composite Functions"
prevcontenturl: ../1.3-combining-functions
nextcontenturl: ../1.6-graph-of-functions
---

Another method of combining functions is by **composition**, where a function contains another function. To visualize this, let's say you want again an apple juice, but this time you want to pack it in a can, so you'll need an additional canning machine. Let's name the juicer $g$, the canning machine $f$, and the apple $x$. If we place the apple to the juicer, we'll get an apple juice $g(x)$, and further placing this in the canning machine, we would get a canned apple juice $f(g(x))$. 



{% include images.html 
    url= "DC/DC-1.4.1.png" 
    caption= "Figure 1"
    size= "90%"
%}



If $f$ and $g$ are both functions of $x$, where $f$ is the outer function and $g$ is the inner function ($f$ is composed with $g$), the composite function is denoted as $(f \circ g)(x)=f(g(x))$, which is read as ``$f$ of $g$ of $x$''.

{% include tcolorbox.html 
    details= "
	(f \circ g)(x)=f(g(x))
    "
%}


For example, given two functions $f(x)=2x+5$ and $g(x)=3x-4$, determine $(f \circ g)(x)$

$$
\begin{align*}
	(f \circ g)(x) &= f(g(x))
\end{align*}
$$

Start with the outer function $f$,

$$
\begin{align*}
	f(x) &= 2x+5 \\
\end{align*}
$$

Then replace $x$ with $g(x)$,

$$
\begin{align*}
	f( \tcA{g(x)} ) &= 2(\tcA{g(x)}) + 5
\end{align*}
$$

Since $g(x)=3x-4$,

$$
\begin{align*}
	f(\tcA{g(x)}) &= 2(\tcA{3x-4}) + 5 \\
	&= 6x-8+5 \\
	&= 6x-3
\end{align*}
$$

Hence, $(f \circ g)= 6x-3$

---
$\example{1}$
If $ f(x)=x^2 $ and $ g(x)=x+1 $, find:
**a.** $ (f \circ g)(x) $,
**b.** $ (g \circ f)(x) $,
**c.** $ (f \circ f)(x) $,
**d.** $ (g \circ g)(x) $



$\solution$ \\
$\For{a}$ \\
$$
\begin{align*}
	(f \circ g)(x) &=  f(g(x)) \\ 
	f(x) &= x^2 \\
	f(g(x)) &=	[g(x)]^2 \\
	&= (x+1)^2 \\
	&= x^2+2x+1		\tagans
\end{align*} 
$$


$\For{b}$ \\
$$
\begin{align*}
	(g \circ f)(x) &=  g(f(x)) \\
	g(x) &= x+1 \\
	g(f(x)) &= f(x)+1\\
	&= x^2+1			\tagans
\end{align*} 
$$


$\For{c}$ \\
$$
\begin{align*}
	(f \circ f)(x) &=  f(f(x)) \\
	f(x) &= x^2 \\
	f(f(x)) &= [f(x)]^2 \\
	&= (x^2)^2 \\
	&= x^4			\tagans
\end{align*} 
$$


$\For{d}$ \\
$$
\begin{align*}
	(g \circ g)(x) &=  g(g(x)) \\
	g(x) &= x+1 \\
	g(g(x)) &= [g(x)]+1 \\
	&= (x+1)+1 \\
	&= x+2			\tagans
\end{align*} 
$$

	
---
$\example{2}$ 
If $ g(x)= 2x+1$ and $ h(x)=3-x^2$, find:
**a.** $ g(h(0)) $,
**b.** $ h(g(2)) $,
**c.** $ g(g(-3)) $,
**d.** $ h(h(1/2)) $

$\solution$ \\
$\For{a}$ \\
$$
\begin{align*}
	g(x) &= 2x+1 \\
	g(h(x)) &= 2(3-x^2)+1 \\
	g(h(0)) &= 2[3-(0)^2]+1 \\
	&= 2(3)+1 \\
	&= 7		\tagans
\end{align*} 
$$


$\For{b}$ \\
$$
\begin{align*}
	h(x) &= 3-x^2 \\
	h(g(x)) &= 3-(2x+1)^2 \\
	h(g(2)) &= 3-[2(2)+1]^2 \\
	&= 3-(5)^2 \\
	&= -22	\tagans
\end{align*} 
$$


$\For{c}$ \\
$$
\begin{align*}
	g(x) &= 2x+1 \\
	g(g(x)) &= 2(2x+1)+1 \\
	g(g(-3)) &= 2[2(-3)+1]+1 \\
	&= 2(-5)+1 \\
	&= -9	\tagans
\end{align*} 
$$


$\For{d}$ \\
$$
\begin{align*}
	h(x) &= 3-x^2 \\
	h(h(x)) &= 3-(3-x^2)^2 \\
	h(h(1/2)) &= 3-[3-(1/2)^2]^2 \\
	&= 3-\br{ 3-\frac{1}{4} }^2 \\
	&= 3-\br{ \frac{11}{4} }^2 \\
	&= -\frac{73}{16}	\tagans
\end{align*} 
$$


---
$\example{3}$
If $ f(x)=x+3$, $ g(x)=(x+1)^2$ and $ h(x)=\frac{1}{x}$, find:
**a.** $ f(g(h(x))) $,
**b.** $ g(h(f(x))) $,
**c.** $ h(f(g(2))) $,
**d.** $ h(g(f(x))) $,
**e.** $ f(h(g(x))) $,
**f.** $ g(f(h(1/2))) $


$\solution$ \\
$\For{a}$ \\
$$
\begin{align*}
	f(x) &= x+3 \\
	f(g(x)) &= (x+1)^2+3 \\
	f(g(h(x))) &= \br{ \frac{1}{x}+1 }^2+3 \\
	&= \br{ \frac{1}{x^2}+\frac{2}{x}+1 }+3 \\
	&= \frac{1}{x^2}+\frac{2}{x}+4	\tagans
\end{align*} 
$$


$\For{b}$ \\
$$
\begin{align*}
	g(x) &= (x+1)^2 \\
	g(h(x)) &= \br{ \frac{1}{x}+1 }^2 \\
	g(h(f(x))) &= \br{ \frac{1}{x+3}+1 }^2 \\
	&= \br{ \frac{1}{x+3}+\frac{x+3}{x+3} }^2 \\
	&= \br{ \frac{x+4}{x+3} }^2 \\    
	&= \frac{(x+4)^2}{(x+3)^2}	\tagans
\end{align*} 
$$


$\For{c}$ \\
$$
\begin{align*}
	h(x) &= \frac{1}{x} \\
	h(f(x)) &= \frac{1}{x+3} \\
	h(f(g(x))) &= \frac{1}{(x+1)^2+3} \\
	h(f(g(2))) &= \frac{1}{(2+1)^2+3} \\
	&= \frac{1}{12}			\tagans
\end{align*} 
$$


$\For{d}$ \\
$$
\begin{align*}
	h(x) &= \frac{1}{x} \\
	h(g(x)) &= \frac{1}{(x+1)^2} \\
	h(g(f(x))) &= \frac{1}{[(x+3)+1]^2} \\
	&= \frac{1}{(x+4)^2}		\tagans
\end{align*} 
$$


$\For{e}$ \\
$$
\begin{align*}
	f(x) &= x+3 \\
	f(h(x)) &= \frac{1}{x}+3 \\
	f(h(g(x))) &= \frac{1}{(x+1)^2}+3  \\
	&= \frac{1+3(x+1)^2}{(x+1)^2} \\
	&= \frac{1+3(x^2+2x+1)}{\left(x+1\right)^2} \\
	&= \frac{3x^2+6x+4}{\left(x+1\right)^2}	\tagans
\end{align*} 
$$


$\For{f}$ \\
$$
\begin{align*}
	g(x) &= (x+1)^2 \\
	g(f(x)) &= (x+3+1)^2 \\
	g(f(h(x))) &= \br{ \frac{1}{x}+4 }^2  \\
	g(f(h(1/2))) &= \br{ \frac{1}{\frac{1}{2}}+4 }^2  \\
	&= (2+4)^2 \\
	&= 36		\tagans
\end{align*} 
$$




---	
$\example{4}$
If $ f(x)= \frac{2}{x+1}$ and $ f(g(x))=x$, determine $g(x)$.

$\solution$ \\
In this case, the composed function is one of the given,  
$$
\begin{align*}
	f(g(x)) &= x
\end{align*}
$$

Start with $f(x)$

$$
\begin{align*}
	f(x) &= \frac{2}{x+1} \\
	f(g(x)) &= \frac{2}{ g(x) +1}
\end{align*}
$$

Since $f(g(x))=x$,

$$
\begin{align*}
	\frac{2}{ g(x) +1} &= x \\
	g(x) +1 &= \frac{2}{x} \\
	g(x) &= \frac{2}{x} -1		\tag*{(ans.)}
\end{align*}
$$

You can check your answer by composing the function,

$$
\begin{align*}
	f(x) &= \frac{2}{x+1} \\
	f(g(x)) &= 	\frac{2}{\br{ \frac{2}{x} -1 }+1} \\
	&= \frac{2}{\frac{2}{x}} \\
	&= x
\end{align*}
$$